gimli/proof/eclib/JWord.ec
@@ -15,19 +15,19 @@ op rflags_of_mul (ov : bool) =
   let ZF = undefined_flag in
   (OF, CF, SF, PF, ZF).
 
-op rflags_undefined = 
+op rflags_undefined =
   let OF = undefined_flag in
   let CF = undefined_flag in
-  let SF = undefined_flag in 
+  let SF = undefined_flag in
   let PF = undefined_flag in
   let ZF = undefined_flag in
   (OF, CF, SF, PF, ZF).
 
-op flags_w (fs:bool * bool * bool * bool * bool) (w : 't) = 
+op flags_w (fs:bool * bool * bool * bool * bool) (w : 't) =
   let (OF, CF, SF, PF, ZF) = fs in
   (OF, CF, SF, PF, ZF, w).
 
-op flags_w2 (fs:bool * bool * bool * bool * bool) (w1 w2: 't) = 
+op flags_w2 (fs:bool * bool * bool * bool * bool) (w1 w2: 't) =
   let (OF, CF, SF, PF, ZF) = fs in
   (OF, CF, SF, PF, ZF, w1, w2).
 
@@ -86,7 +86,8 @@ proof. smt (ge2_modulus). qed.
 lemma max_size : max 0 size = size.
 proof. by rewrite /max gt0_size. qed.
 
-hint exact : ge0_size gt0_size gt0_modulus ge2_modulus ge0_modulus max_size.
+hint exact : ge0_size gt0_size max_size.
+hint [rigid] exact : gt0_modulus ge2_modulus ge0_modulus.
 
 lemma half_modulus : 2 ^ (size -1) = modulus %/ 2.
 proof. rewrite (expr_pred 2 size) // /#. qed.
@@ -184,7 +185,7 @@ op all_words = map of_int (iota_ 0 modulus)
 axiomatized by all_wordsE.
 
 lemma all_wordsP x : x \in all_words.
-proof. 
+proof.
   rewrite all_wordsE mapP; exists (to_uint x).
   by rewrite mema_iota /= to_uint_cmp.
 qed.
@@ -221,6 +222,18 @@ qed.
 lemma zerowE i: zero.[i] = false.
 proof. by rewrite of_intwE /int_bit. qed.
 hint simplify zerowE.
+
+lemma nth_one i : one.[i] = (i = 0).
+proof.
+  rewrite of_intwE /int_bit (modz_small 1).
+  + smt(ge2_modulus).
+  case: (i = 0); first by move => -> />; rewrite gt0_size.
+  case: (0 <= i); last done.
+  move => ?? /=.
+  suff -> : 1 %/ 2 ^ i = 0 by done.
+  apply: divz_small => />.
+  smt(expr_gt0 powS_minus).
+qed.
 
 lemma of_int_powm1 p i :
   0 <= p =>
@@ -276,10 +289,13 @@ proof.
   rewrite modzMDl !modz_pow2_div; 1,2:smt().
   have -> : i + j + 1 - (i + j) = 1 by ring.
   have -> : i + j - i = j by ring.
-  rewrite (exprD_nneg 2 j 1) 1,2:// pow2_1 (modz_small _ (2^j * 2)).
-  + apply bound_abs; split => [|?]; 1: smt (modz_cmp to_uint_cmp gt0_pow2).
-    by rewrite -hrec; smt (modz_cmp to_uint_cmp gt0_pow2).
-  by rewrite addzC mulzC b2i_get 1:/#.
+  rewrite (exprD_nneg 2 j 1) 1,2:// pow2_1.
+  rewrite addzC mulzC b2i_get 1:/#.
+  rewrite (modz_small _ (2^j * 2)); last by [].
+  move: (to_uint w) => z.
+  split; 1: smt (modz_cmp gt0_pow2).
+  have -> : `|2^j*2| = 2^j + 2^j by smt(gt0_pow2).
+  rewrite addzC ltr_le_add; smt (modz_cmp gt0_pow2).
 qed.
 
 lemma bitsE w k len : bits w k len = mkseq (fun (i:int) => w.[k+i]) len.
@@ -540,7 +556,7 @@ op ulift2 (f : int -> int -> int) (w1 w2 : t) =
   of_int (f (to_uint w1) (to_uint w2)).
 
 op slift2 (f : int -> int -> int) (w1 w2 : t) =
-  of_int (f (to_uint w1) (to_uint w2)).
+  of_int (f (to_sint w1) (to_sint w2)).
 
 op ( + ) = ulift2 Int.( + ) axiomatized by addE.
 op ([-]) = ulift1 Int.([-]) axiomatized by oppE.
@@ -549,9 +565,8 @@ op ( * ) = ulift2 Int.( * ) axiomatized by mulE.
 op (\udiv) = ulift2 IntDiv.( %/) axiomatized by udivE.
 op (\umod) = ulift2 IntDiv.( %%) axiomatized by umodE.
 
-(* TODO check this *)
-op (\sdiv) = slift2 IntDiv.( %/) axiomatized by sdivE.
-op (\smod) = slift2 IntDiv.( %%) axiomatized by smodE.
+op (\sdiv) = slift2 (\zquot) axiomatized by sdivE.
+op (\smod) = slift2 (\zrem) axiomatized by smodE.
 
 (* --------------------------------------------------------------------- *)
 (* Comparisons                                                           *)
@@ -763,18 +778,49 @@ lemma to_sint_unsigned (x : t) : 0 <= to_sint x => to_sint x = to_uint x.
 proof. smt(to_sintE to_uint_cmp). qed.
 
 lemma to_sintK_small i : min_sint <= i <= max_sint => to_sint (of_int i) = i.
-proof. rewrite of_sintK /smod half_modulus /#. qed.
+proof.
+  rewrite of_sintK /smod half_modulus.
+  have := modz_cmp i modulus.
+  smt().
+qed.
 
 lemma to_sintD_small (a b : t):
   min_sint <= to_sint a + to_sint b <= max_sint =>
   to_sint (a + b) = to_sint a + to_sint b.
-proof. rewrite !to_sintE to_uintD /smod /= half_modulus /#. qed.
+proof.
+  rewrite !to_sintE to_uintD /smod /= half_modulus.
+  have := modz_cmp (to_uint a + to_uint b) modulus.
+  smt().
+qed.
 
 lemma to_sintB_small (a b : t):
   min_sint <= to_sint a - to_sint b <= max_sint =>
   to_sint (a - b) = to_sint a - to_sint b.
-proof. rewrite !to_sintE /smod /= half_modulus to_uintD to_uintN modzDmr /#. qed.
+proof.
+  rewrite !to_sintE /smod /= half_modulus to_uintD to_uintN modzDmr.
+  have := modz_cmp (to_uint a - to_uint b) modulus gt0_modulus.
+  have := to_uint_cmp a.
+  have := to_uint_cmp b.
+  smt().
+qed.
 
+lemma to_uintBb x y c :
+  to_uint (x - (y + of_int (b2i c))) = to_uint x - to_uint y - b2i c + modulus * b2i (to_uint x < to_uint y + b2i c).
+proof.
+have /= x_range := to_uint_cmp x.
+have /= y_range := to_uint_cmp y.
+rewrite /b2i to_uintD.
+case: c => _; last first.
++ rewrite to_uintN !addr0 modzDmr.
+  case: (to_uint x < to_uint y) => Hxy /=.
+  + rewrite (addzC (to_uint x - to_uint y) modulus).
+    by rewrite &(modz_sub_carry) // subz_lt0 //.
+  + by rewrite pmod_small /#.
+rewrite to_uintN.
+case: (to_uint y = max_uint) => /= hy.
++ rewrite to_uintD hy /#.
+rewrite to_uintD_small ?modNz // /#.
+qed.
 
 (* --------------------------------------------------------------------- *)
 (* Ring tactic                                                           *)
@@ -823,40 +869,7 @@ op subc (x y:t) (b: bool): bool * t = (borrow_sub x y b, x-(y+of_int (b2i b)))
 lemma subcP x y c:
  let (c',z) = subc x y c
  in to_uint z - modulus * b2i c' = to_uint x - (to_uint y + b2i c).
-proof.
-rewrite subcE /borrow_sub /=.
-case: (to_uint y + b2i c = modulus) => H.
- rewrite to_uintD.
- have -> /=: to_uint (- (y + of_int (b2i c))) = 0.
-  rewrite to_uintN to_uintD of_uintK (modz_small (b2i c)).
-   by apply bound_abs; smt(ge2_modulus).
-  by rewrite H modzz /=.
- rewrite H modz_small.
-  by apply bound_abs; apply to_uint_cmp.
- have ->: to_uint x < modulus by smt(to_uint_cmp).
- smt().
-case: (to_uint x < to_uint y + b2i c) => ?/=.
- have E: to_uint y + b2i c = to_uint (y + of_int (b2i c)).
-  rewrite to_uintD_small.
-   rewrite !of_uintK modz_small; first by  apply bound_abs; smt(ge2_modulus).
-   by case: c => /=?; smt(to_uint_cmp).
-  by rewrite of_uintK modz_small //; apply bound_abs; smt(ge2_modulus).
- rewrite E b2i1 /= eqr_sub.
- have ->: x - (y + of_int (b2i c)) = -((y + of_int (b2i c)) - x) by ring.
- rewrite to_uintN -modzDl modz_small.
-  have ?: 0 < to_uint (y + of_int (b2i c) - x) <= `|modulus|.
-   rewrite to_uintB; first by rewrite uleE -E; smt().
-   rewrite -E; smt(to_uint_cmp).
-  smt(to_uint_cmp).
- rewrite to_uintB; first by rewrite uleE -E; smt().
- smt(to_uint_cmp).
-rewrite b2i0 /= to_uintB.
- rewrite uleE to_uintD_small.
-  by rewrite of_uintK modz_small; smt(to_uint_cmp ge2_modulus).
- rewrite of_uintK modz_small; first smt(ge2_modulus).
- smt(ge2_modulus to_uint_cmp).
-by rewrite to_uintD of_uintK !modz_small; smt(ge2_modulus to_uint_cmp).
-qed.
+proof. rewrite subcE /borrow_sub /= to_uintBb /#. qed.
 
 abbrev subc_borrow x y c = (subc x y c).`1.
 
@@ -1212,7 +1225,7 @@ rewrite andwC => ?; have: to_uint (invw y `&` x) = 0 by smt(to_uint0).
 rewrite !to_uintE andE invE => ?.
 have ->: x \ule y = (0 <= (to_uint y - to_uint x)) by rewrite uleE /#.
 rewrite !to_uintE; apply bs2int_sub_common.
-+ by rewrite !size_w2bits. 
++ by rewrite !size_w2bits.
 by rewrite map_w2bits_w2bits map2_w2bits_w2bits.
 qed.
 
@@ -1301,15 +1314,15 @@ lemma masklsbE k i:
  (masklsb k).[i] = 0 <= i < min k size.
 proof.
 case: (0 <= k) => H; last first.
-+ by rewrite ler_maxl 1:/# /=; smt(ge0_size). 
-rewrite ler_maxr 1://. 
++ by rewrite ler_maxl 1:/# /=; smt(ge0_size).
+rewrite ler_maxr 1://.
 case: (0 <= i < size) => Hi; last by rewrite get_out /#.
 rewrite of_intE.
 case: (size <= k) => H0.
 + rewrite powm1_mod // get_bits2w //.
   have /=:= (bs2int_nseq true size); rewrite ge0_size /= => <-.
   have:= bs2intK (nseq size true); rewrite size_nseq ler_maxr 1:/# => ->.
-  by rewrite nth_nseq //#. 
+  by rewrite nth_nseq //#.
 rewrite modz_small; first by smt(gt0_pow2 ler_weexpn2l).
 rewrite get_bits2w //.
 have /= := (bs2int_nseq true k); rewrite H /= => <-.
@@ -1461,7 +1474,7 @@ move=> *.
 by apply (ler_lt_trans (to_uint w)); smt(leq_trunc_div gt0_pow2 to_uint_cmp).
 qed.
 
-op wmulhs (v1 v2: t) = 
+op wmulhs (v1 v2: t) =
   of_int (to_sint v1 * to_sint v2 %/ modulus).
 
 theory ALU.
@@ -1482,7 +1495,7 @@ op ZF_of (w : t) = w = zero.
 op rflags_of_bwop (w : t) =
   let OF = false in
   let CF = false in
-  let SF = SF_of w in 
+  let SF = SF_of w in
   let PF = undefined_flag in
   let ZF = ZF_of w in
   (OF, CF, SF, PF, ZF).
@@ -1527,8 +1540,8 @@ op rflags_of_bwop_w (w : t) =
 op set0_XX_ = (false,false,false,false,false, of_int 0).
 
 op ADD_XX (v1 v2 : t)  =
-  rflags_of_aluop_w 
-    (v1 + v2) 
+  rflags_of_aluop_w
+    (v1 + v2)
     (to_uint v1 + to_uint v2)
     (to_sint v1 + to_sint v2).
 
@@ -1589,7 +1602,7 @@ op IDIV_XX (hi lo dv: t) =
 (* Same comment than for DIV_XX *)
 (*let ov = (q <? wmin_signed sz)%Z || (q >? wmax_signed sz)%Z in
   let (q, r) = if dv = 0 || ov then (0,0) else (q, r) in *)
-  flags_w2 rflags_undefined (of_int q) (of_int r). 
+  flags_w2 rflags_undefined (of_int q) (of_int r).
 
 op CQO_XX (w:t) =
   of_int (if SF_of w then -1 else 0).
@@ -1649,9 +1662,9 @@ op TEST_XX (x y: t) =
   rflags_of_bwop (x `&` y).
 
 op CMP_XX (x y: t) =
-  rflags_of_aluop 
+  rflags_of_aluop
      (x - y)
-     (to_uint x - to_uint y) 
+     (to_uint x - to_uint y)
      (to_sint x - to_sint y).
 
 op AND_XX (v1 v2: t) =
@@ -1677,6 +1690,10 @@ op LZCNT_XX (w:t) =
 op TZCNT_XX (w:t) =
   let v = of_int (lzcnt (w2bits w)) in
   (undefined_flag, ZF_of w, undefined_flag, undefined_flag, ZF_of v, v).
+
+op BSR_XX (w: t) =
+  (undefined_flag, undefined_flag, undefined_flag, undefined_flag, false,
+   of_int (size - 1 - lzcnt (w2bits w))).
 
 lemma DEC_XX_counter n (c:t) :
   c <> zero =>
@@ -1726,13 +1743,13 @@ theory W8.
   rename [op, lemma] "_XX" as "_8"
   proof gt0_size by done.
 
-  op (`>>`) (w1 w2 : W8.t) = w1 `>>>` (to_uint w2 %% size).
-  op (`|>>`) (w1 w2 : W8.t) = w1 `|>>>` (to_uint w2 %% size).
-  op (`<<`) (w1 w2 : W8.t) = w1 `<<<` (to_uint w2 %% size).
+  op (`>>`) (w1 w2 : W8.t) = w1 `>>>` to_uint w2.
+  op (`|>>`) (w1 w2 : W8.t) = w1 `|>>>` to_uint w2.
+  op (`<<`) (w1 w2 : W8.t) = w1 `<<<` to_uint w2.
 
-  lemma shr_div w1 w2 : to_uint (w1 `>>` w2) = to_uint w1 %/ 2^ (to_uint w2 %% size).
+  lemma shr_div w1 w2 : to_uint (w1 `>>` w2) = to_uint w1 %/ 2^ to_uint w2.
   proof.
-    rewrite -{1}(to_uintK w1) /(`>>`) shrDP; 1: smt (modz_cmp).
+    rewrite -{1}(to_uintK w1) /(`>>`) shrDP; 1: smt (to_uint_cmp).
     rewrite of_uintK to_uint_mod modz_small 2://.
     apply bound_abs; apply divz_cmp; 1: by apply gt0_pow2.
     by have:= to_uint_cmp w1; smt (gt0_pow2).
@@ -1742,18 +1759,17 @@ theory W8.
        to_uint (w1 `>>` (of_int i)) = to_uint w1 %/ 2^i.
   proof.
     move=> hi;rewrite shr_div of_uintK.
-    rewrite (modz_small i);1: smt (pow2_8).
-    by rewrite modz_small.
+    by rewrite (modz_small i);1: smt (pow2_8).
   qed.
 
-  op (`|>>|`) (w1 w2 : W8.t) = w1 `|>>>|` (to_uint w2 %% size).
-  op (`|<<|`) (w1 w2 : W8.t) = w1 `|<<<|` (to_uint w2 %% size).
+  op (`|>>|`) (w1 w2 : W8.t) = w1 `|>>>|` to_uint w2.
+  op (`|<<|`) (w1 w2 : W8.t) = w1 `|<<<|` to_uint w2.
 
   lemma rol_xor_shft w i : 0 < i < size =>
     w `|<<<|` i = (w `<<` of_int i) +^ (w `>>` of_int (size - i)).
   proof.
     move=> hi; rewrite /(`<<`) /(`>>`) !of_uintK /=.
-    by rewrite !(modz_small _ 256) 1,2:/# !modz_small 1,2:/# rol_xor 1:/#.
+    by rewrite !(modz_small _ 256) 1,2:/# rol_xor 1:/#.
   qed.
 
   op SETcc (b: bool) = b ? W8.one : W8.zero.
@@ -1761,17 +1777,17 @@ theory W8.
   theory SHIFT.
 
   op shift_mask i = to_uint i %% 32.
-  
+
   op ROR_8 (v: t) (i: W8.t) =
     let i = shift_mask i in
-    if i = 0 then (undefined_flag, undefined_flag, v) 
+    if i = 0 then (undefined_flag, undefined_flag, v)
     else
       let r = v `|>>>|` i in
       let CF = ALU.SF_of r in
       let OF = if i = 1 then CF <> ALU.SF_of v else undefined_flag in
       (OF , CF,  r)
   axiomatized by ROR_8_E.
-  
+
   op ROL_8 (v: t) (i: W8.t) =
     let i = shift_mask i in
     if i = 0 then(undefined_flag, undefined_flag, v)
@@ -1781,8 +1797,8 @@ theory W8.
       let OF = if i = 1 then ALU.SF_of r <> CF else undefined_flag in
       (OF, CF, r)
   axiomatized by ROL_8_E.
-  
-  op im i = 
+
+  op im i =
     if size = 8 then i %% 9
     else if size = 16 then i %% 17
     else i.
@@ -1792,18 +1808,18 @@ theory W8.
     let im = im i in
     let r  = fun j => if j = 0 then cf else v.[j-1] in
     let r  = fun j => r ((j - i) %% 9) in
-    let CF = r 0 in 
+    let CF = r 0 in
     let r  = init (fun j => r (j+1)) in
     let OF = if i = 1 then (ALU.SF_of r <> CF) else undefined_flag in
     (OF, CF, r).
-  
+
   op RCR_8 (v: t) (i: W8.t) (cf:bool) =
     let i  = shift_mask i in
     let im = im i in
     let r  = fun j => if j = 0 then cf else v.[j-1] in
     let r  = fun j => r ((j + i) %% 9) in
     let OF = if i = 1 then ALU.SF_of  v <> cf else undefined_flag in
-    let CF = r 0 in 
+    let CF = r 0 in
     let r  = init (fun j => r (j+1)) in
     (OF, CF, r).
 
@@ -1819,7 +1835,7 @@ theory W8.
     let i = shift_mask i in
     if i = 0 then flags_w rflags_undefined v
     else
-      let rc = ALU.SF_of (v `<<<` (i - 1)) in 
+      let rc = ALU.SF_of (v `<<<` (i - 1)) in
       let r  = v `<<<` i in
       rflags_OF i r rc (ALU.SF_of r ^^ rc).
 
@@ -1832,15 +1848,15 @@ theory W8.
       let r2 = v2 `>>>` (size - i) in
       let r  = r1 +^ r2 in
       rflags_OF i r rc (ALU.SF_of r ^^ rc).
-  
+
   op SHR_8 (v: t) (i: W8.t) =
-    let i = shift_mask i in 
-    if i = 0 then flags_w rflags_undefined v 
+    let i = shift_mask i in
+    if i = 0 then flags_w rflags_undefined v
     else
       let rc = lsb (v `>>>` i -1) in
       let r  = v `>>>` i in
       rflags_OF i r rc (ALU.SF_of r).
-  
+
   op SHRD_8 (v1 v2: t) (i: W8.t) =
     let i = shift_mask i in
     if i = 0 then flags_w rflags_undefined v1
@@ -1878,7 +1894,7 @@ abstract theory WT.
   op wmulhs : t -> t -> t.
 
   op (+) : t -> t -> t.
-  op [-] : t -> t. 
+  op [-] : t -> t.
   op ( * ) : t -> t -> t.
 
   op (`>>>`) : t -> int -> t.
@@ -1892,11 +1908,15 @@ abstract theory WT.
   op to_uint : t -> int.
   op to_sint : t -> int.
 
+  op onew  = of_int (2^size - 1).
+
   op bits : t -> int -> int -> bool list.
 
   abbrev (`|<<<|`) = rol.
 
   axiom initiE (f : int -> bool) (i : int) : 0 <= i < size => (init f).[i] = f i.
+
+  axiom onewE (i : int) : onew.[i]  = (0<= i < size).
 
   axiom andwE (w1 w2 : t) (i : int) : (andw w1 w2).[i] = (w1.[i] /\ w2.[i]).
   axiom orwE  (w1 w2 : t) (i : int) : (orw  w1 w2).[i] = (w1.[i] \/ w2.[i]).
@@ -1947,15 +1967,15 @@ abstract theory BitWordSH.
   op shift_mask i =
     W8.to_uint i %% (if size <= 32 then 32 else size).
 
-  op (`>>`) (w1 : t) (w2 : W8.t) = w1 `>>>` (to_uint w2 %% size).
-  op (`<<`) (w1 : t) (w2 : W8.t) = w1 `<<<` (to_uint w2 %% size).
-  op (`|>>`) (w1 : t) (w2 : W8.t) = w1 `|>>>` (to_uint w2 %% size).
-  op (`|>>|`) (w1 : t) (w2 : W8.t) = w1 `|>>>|` (to_uint w2 %% size).
-  op (`|<<|`) (w1 : t) (w2 : W8.t) = w1 `|<<<|` (to_uint w2 %% size).
+  op (`>>`) (w1 : t) (w2 : W8.t) = w1 `>>>` to_uint w2.
+  op (`<<`) (w1 : t) (w2 : W8.t) = w1 `<<<` to_uint w2.
+  op (`|>>`) (w1 : t) (w2 : W8.t) = w1 `|>>>` to_uint w2.
+  op (`|>>|`) (w1 : t) (w2 : W8.t) = w1 `|>>>|` to_uint w2.
+  op (`|<<|`) (w1 : t) (w2 : W8.t) = w1 `|<<<|` to_uint w2.
 
-  lemma shr_div w1 w2 : to_uint (w1 `>>` w2) = to_uint w1 %/ 2^ (to_uint w2 %% size).
+  lemma shr_div w1 w2 : to_uint (w1 `>>` w2) = to_uint w1 %/ 2^ to_uint w2.
   proof.
-    rewrite -{1}(to_uintK w1) /(`>>`) shrDP; 1: smt (modz_cmp gt0_size).
+    rewrite -{1}(to_uintK w1) /(`>>`) shrDP; 1: smt(W8.to_uint_cmp).
     rewrite of_uintK to_uint_mod modz_small 2://.
     apply bound_abs; apply divz_cmp; 1: by apply gt0_pow2.
     by have:= to_uint_cmp w1; smt (gt0_pow2).
@@ -1965,8 +1985,7 @@ abstract theory BitWordSH.
      to_uint (w1 `>>` (W8.of_int i)) = to_uint w1 %/ 2^ i.
   proof.
     move=> hi;rewrite shr_div of_uintK.
-    rewrite (modz_small i) 1:pow2_8; 1: smt (size_le_256).
-    by rewrite modz_small //;apply bound_abs.
+    by rewrite (modz_small i) 1:pow2_8; 1: smt (size_le_256).
   qed.
 
   lemma rol_xor_shft w i : 0 < i < size =>
@@ -1975,7 +1994,7 @@ abstract theory BitWordSH.
     move=> hi; rewrite /(`<<`) /(`>>`) !W8.of_uintK.
     have h : 0 <= i < `|W8.modulus|.
     + by rewrite /=; smt (size_le_256).
-    rewrite !(modz_small _ W8.modulus) 1:// 1: #smt: (size_le_256) !modz_small 1,2:/#.
+    rewrite !(modz_small _ W8.modulus) 1:// 1: #smt: (size_le_256).
     by rewrite rol_xor 1:/#.
   qed.
 
@@ -1983,18 +2002,14 @@ abstract theory BitWordSH.
    0 <= k < size =>
    w `<<` W8.of_int k = w `<<<` k.
   proof.
-   move=> *; rewrite /(`<<`) of_uintK (modz_small (k %% W8.modulus)).
-    smt(modz_cmp).
-   by rewrite modz_small //; smt(size_le_256).
+    move=> *; rewrite /(`<<`) of_uintK modz_small //; smt(size_le_256).
   qed.
 
   lemma shr_shrw k w:
    0 <= k < size =>
    w `>>` W8.of_int k = w `>>>` k.
   proof.
-   move=> *; rewrite /(`>>`) of_uintK (modz_small (k %% W8.modulus)).
-    smt(modz_cmp).
-   by rewrite modz_small //; smt(size_le_256).
+    move=> *; rewrite /(`>>`) of_uintK modz_small //; smt(size_le_256).
   qed.
 
   theory SHIFT.
@@ -2211,7 +2226,7 @@ abstract theory W_WS.
     Pack.init (fun i => w \bits'S i)
   axiomatized by unpack'SE.
 
-  abbrev to_list (w:WB.t) : WS.t list = 
+  abbrev to_list (w:WB.t) : WS.t list =
     map ((\bits'S) w) (iotared 0 r).
 
   op pack'R_t (ws:pack_t) =
@@ -2219,6 +2234,9 @@ abstract theory W_WS.
   axiomatized by pack'RE.
 
   abbrev pack'R (ws:WS.t list) = pack'R_t (Pack.of_list ws).
+
+  lemma size_to_list (w:WB.t) : size (to_list w) = r.
+  proof. by rewrite size_map iotaredE size_iota /max gt0_r. qed.
 
   lemma pack'RwE (ws:pack_t) i : 0 <= i < sizeB =>
     (pack'R_t ws).[i] = ws.[i %/ sizeS].[i %% sizeS].
@@ -2244,13 +2262,23 @@ abstract theory W_WS.
      w \bits'S i = WS.of_int 0.
   proof.
     move=> hi;apply WS.wordP => k hk.
-    rewrite bits'SiE 1:// WS.of_intwE /WS.int_bit /= get_to_uint sizeBrS /#.
+    rewrite bits'SiE 1:// WS.of_intwE /WS.int_bit /= get_to_uint sizeBrS.
+    pose x := _ && _; have -> : x = false; last by [].
+    have : (i < 0) \/ (r <= i) by smt().
+    case => ?; first smt().
+    suff : r * sizeS <= i * sizeS + k; smt().
   qed.
 
   lemma get_zero i : WB.of_int 0 \bits'S i = WS.of_int 0.
   proof.
     apply WS.wordP => k hk.
     by rewrite bits'SiE 1:// WS.of_intwE /WS.int_bit /= get_to_uint /= WB.of_uintK.
+  qed.
+
+  lemma _m_one_bits8 i :  0 <= i < r => (WB.of_int (2^sizeB - 1))  \bits'S i = WS.onew.
+  proof.
+    move => *. apply WS.wordP. move => j h.
+    by rewrite bits'SiE //  WB.onewE WS.onewE h in_bound //.
   qed.
 
   lemma unpack'SK w : pack'R_t (unpack'S w) = w.
@@ -2277,9 +2305,9 @@ abstract theory W_WS.
   qed.
 
   lemma allP (w1 w2 :WB.t) : all (fun i => w1 \bits'S i = w2 \bits'S i) (iotared 0 r) => w1 = w2.
-  proof. 
+  proof.
     rewrite allP => h; apply wordP => i hi; apply h.
-    by rewrite iotaredE (mema_iota 0 r). 
+    by rewrite iotaredE (mema_iota 0 r).
   qed.
 
   op map (f:WS.t -> WS.t) (w:WB.t) =
@@ -2302,50 +2330,66 @@ abstract theory W_WS.
     by move=> hi;rewrite map2E pack'RbE // map2iE // !unpack'SE !initiE.
   qed.
 
-  lemma map_pack'R f ws : 
+  lemma map_pack'R f ws :
     map f (pack'R ws) = pack'R (mapN f (WS.of_int 0) ws r).
-  proof. 
+  proof.
     apply wordP => i hi.
     by rewrite mapbE 1:// pack'RbE 1:// pack'RbE 1:// -map_of_list mapiE.
   qed.
 
-  lemma nth_to_list w i : 
+  lemma nth_to_list_in w i :
     0 <= i < r =>
     nth (WS.of_int 0) (to_list w) i = w \bits'S i.
   proof.
-    move=> hi; rewrite iotaredE (nth_map 0) 1:size_iota /max 1:gt0_r 1:// nth_iota //. 
+    move=> hi; rewrite iotaredE (nth_map 0) 1:size_iota /max 1:gt0_r 1:// nth_iota //.
   qed.
 
-  lemma map_to_list f w : 
-    map f w = pack'R (map f (to_list w)). 
-  proof. 
-    apply wordP => i hi.
-    rewrite mapbE 1:// pack'RbE 1:// get_of_list 1:// iotaredE. 
-    have hs : 0 <= i && i < size (iota_ 0 r) by rewrite size_iota /max gt0_r.
-    rewrite (nth_map (WS.of_int 0)) 1:size_map 1://. 
-    by rewrite (nth_map 0) 1:// nth_iota. 
+  lemma nth_to_list w i :
+    nth (WS.of_int 0) (to_list w) i = w \bits'S i.
+  proof.
+    case: ( 0 <= i < r) => h; first by apply nth_to_list_in.
+    by rewrite nth_out 1:size_to_list // get_out.
   qed.
-    
+
+  lemma get_pack'R (l : WS.t list) (k : int) :
+    size l = r => (pack'R l \bits'S k) = nth (WS.of_int 0) l k.
+  proof.
+    move=> hsz.
+    case: (0 <= k < r) => hk.
+    + by rewrite pack'RbE // Pack.get_of_list.
+    by rewrite nth_out 1:hsz 1:// get_out.
+  qed.
+
+  lemma map_to_list f w :
+    map f w = pack'R (map f (to_list w)).
+  proof.
+    apply wordP => i hi.
+    rewrite mapbE 1:// pack'RbE 1:// get_of_list 1:// iotaredE.
+    have hs : 0 <= i && i < size (iota_ 0 r) by rewrite size_iota /max gt0_r.
+    rewrite (nth_map (WS.of_int 0)) 1:size_map 1://.
+    by rewrite (nth_map 0) 1:// nth_iota.
+  qed.
+
   hint simplify map_pack'R @0, map_to_list @1.
 
-  lemma map2_pack'R f ws1 ws2 : 
+  lemma map2_pack'R f ws1 ws2 :
     map2 f (pack'R ws1) (pack'R ws2) = pack'R (mapN2 f (WS.of_int 0) (WS.of_int 0) ws1 ws2 r).
-  proof. 
+  proof.
     apply wordP => i hi.
     by rewrite map2bE 1:// !pack'RbE 1..3:// -map2_of_list map2iE.
   qed.
 
-  lemma map2_to_list f w1 w2 : 
-    map2 f w1 w2 = pack'R (map2 f (to_list w1) (to_list w2)). 
-  proof. 
+  lemma map2_to_list f w1 w2 :
+    map2 f w1 w2 = pack'R (map2 f (to_list w1) (to_list w2)).
+  proof.
     apply wordP => i hi.
-    rewrite map2bE 1:// pack'RbE 1:// get_of_list 1:// iotaredE. 
+    rewrite map2bE 1:// pack'RbE 1:// get_of_list 1:// iotaredE.
     have hs : 0 <= i && i < size (iota_ 0 r) by rewrite size_iota /max gt0_r.
-    rewrite (nth_map2 (WS.of_int 0) (WS.of_int 0)) 1:size_map 1://. 
+    rewrite (nth_map2 (WS.of_int 0) (WS.of_int 0)) 1:size_map 1://.
     + by rewrite size_map.
-    by rewrite !(nth_map 0) 1,2:// nth_iota. 
+    by rewrite !(nth_map 0) 1,2:// nth_iota.
   qed.
-    
+
   hint simplify map2_pack'R @0, map2_to_list @1.
 
   lemma andb'SE (w1 w2:WB.t) i :
@@ -2511,22 +2555,22 @@ abstract theory W_WS.
      map2 WS.(+) w1 w2.
 
    op VPSUB_'Ru'S (w1 : WB.t) (w2 : WB.t) =
-     map2 (fun (x y:WS.t) => x + (- y)) w1 w2. 
+     map2 (fun (x y:WS.t) => x + (- y)) w1 w2.
 
    op VPMULL_'Ru'S (w1 : WB.t) (w2 : WB.t) =
-     map2 WS.( * ) w1 w2. 
-   
+     map2 WS.( * ) w1 w2.
+
    op VPMULH_'Ru'S (w1 : WB.t) (w2 : WB.t) =
      map2 (fun (x y:WS.t) => wmulhs x y) w1 w2.
 
    op VPSLL_'Ru'S (w : WB.t) (cnt : W128.t) =
-     map (fun (w:WS.t) => w `<<<` (to_uint cnt %% sizeS)) w.
+     map (fun (w:WS.t) => w `<<<` to_uint (W64.of_int (to_uint cnt))) w.
 
    op VPSRL_'Ru'S (w : WB.t) (cnt : W128.t) =
-     map (fun (w:WS.t) => w `>>>` (to_uint cnt %% sizeS)) w.
+     map (fun (w:WS.t) => w `>>>` to_uint (W64.of_int (to_uint cnt))) w.
 
    op VPSRA_'Ru'S (w : WB.t) (cnt : W128.t) =
-     map (fun (w:WS.t) => w `|>>>` (to_uint cnt %% sizeS)) w.
+     map (fun (w:WS.t) => w `|>>>` to_uint (W64.of_int (to_uint cnt))) w.
 
    op VPBROADCAST_'Ru'S (w : WS.t) =
      pack'R (map (fun i => w) (iota_ 0 r)).
@@ -2535,26 +2579,33 @@ abstract theory W_WS.
      if cmp (to_sint x) (to_sint y) then (WS.of_int (-1)) else (WS.of_int 0).
 
    op VPCMPGT_'Ru'S (w1 : WB.t) (w2: WB.t) =
-     map2 (wcmp Int.(<=)) w2 w1.
+     map2 (wcmp Int.(<)) w2 w1.
 
    op VPCMPEQ_'Ru'S (w1 : WB.t) (w2: WB.t) =
      map2 (wcmp (=)) w1 w2.
 
-   op VPMAXU_'Ru'S (w1 : WB.t) (w2 : WB.t) = 
+  op VPSIGN_'Ru'S (w1 : WB.t) (w2 : WB.t) =
+    let sign = fun x => if x < 0 then -1 else if x = 0 then 0 else 1 in
+    map2 (fun x m => x * WS.of_int (sign (WS.to_sint m))) w1 w2.
+
+   op VPMAXU_'Ru'S (w1 : WB.t) (w2 : WB.t) =
      map2 (fun x y => if WS.to_uint x < WS.to_uint y then y else x) w1 w2.
-  
-   op VPMAXS_'Ru'S (w1 : WB.t) (w2 : WB.t) = 
+
+   op VPMAXS_'Ru'S (w1 : WB.t) (w2 : WB.t) =
      map2 (fun x y => if WS.to_sint x < WS.to_sint y then y else x) w1 w2.
-  
-   op VPMINU_'Ru'S (w1 : WB.t) (w2 : WB.t) = 
+
+   op VPMINU_'Ru'S (w1 : WB.t) (w2 : WB.t) =
      map2 (fun x y => if WS.to_uint x < WS.to_uint y then x else y) w1 w2.
 
-   op VPMINS_'Ru'S (w1 : WB.t) (w2 : WB.t) = 
+   op VPMINS_'Ru'S (w1 : WB.t) (w2 : WB.t) =
      map2 (fun x y => if WS.to_sint x < WS.to_sint y then x else y) w1 w2.
+
+   op VPABS_'Ru'S (w: WB.t) =
+     map (fun x => WS.of_int `|WS.to_sint x|) w.
 
    op VPEXTR_'S (w: WB.t) (i: W8.t) = w \bits'S ((W8.to_uint i)%% r).
 
-   op VPINSR_'Ru'S (w1:WB.t) (w2:WS.t) (i:W8.t) : WB.t = 
+   op VPINSR_'Ru'S (w1:WB.t) (w2:WS.t) (i:W8.t) : WB.t =
      pack'R_t (init (fun j => if j = to_uint i %% r then w2 else w1 \bits'S j)).
 
    op VPSLLV_'Ru'S (w1:WB.t) (w2:WB.t) =
@@ -2704,7 +2755,9 @@ proof.
   + have := modz_cmp i n hn.
     have -> : `|n * d| = n * d by smt().
     have -> h : n * d = (n-1) * d + d by ring.
-    split;1: smt(); move=> ?.
+    split.
+    * apply: addz_ge0; smt().
+    move=> ?.
     apply ler_lt_add; 2:smt().
     by rewrite mulzC ler_pmul2r /#.
   by rewrite (divz_small _ (n*d)) 1://  (modz_small _ (n*d)) 1:// /=; ring.
