gimli/proof/eclib/JByte_array.ec
@@ -1,0 +1,451 @@
+(* -------------------------------------------------------------------- *)
+require import AllCore Distr DList BitEncoding IntDiv SmtMap List StdOrder BitEncoding Bool.
+(*---*) import Ring.IntID IntOrder BS2Int.
+require import JUtils JArray JWord.
+
+abstract theory ByteArray.
+
+  clone include MonoArray with
+    type elem <- W8.t,
+    op dfl    <- W8.zero.
+
+  op darray = dmap (dlist W8.dword size) of_list.
+
+  abbrev [-printing] get8  (t:t) (i:int) : W8.t = t.[i].
+  abbrev [-printing] get8d (t:t) (i:int) : W8.t = t.[i].
+
+  abbrev [-printing] set8  (t:t) (i:int) (w:W8.t) : t = t.[i <- w].
+  abbrev [-printing] set8d (t:t) (i:int) (w:W8.t) : t = t.[i <- w].
+
+  abbrev [-printing] of_list8 = of_list.
+
+  op is_init_cell (t:t) (i: int): bool = 0 <= i < size => t.[i] = W8.of_int 255.
+
+  op is_init (t:t) (k l : int): bool = forall i, k <= i => i < k + l => is_init_cell t i.
+
+  op init_arr (b : W8.t) : t =
+    init (fun _ => b).
+
+ lemma init_arrP (t: t) (k: int) : is_init_cell (init_arr (W8.of_int 255))  k.
+ proof. by move => hk; rewrite /is_init_cell initE hk. qed.
+
+ lemma is_init_set_last t len :
+   is_init t 0 len => is_init t.[len <- W8.of_int 255] 0 (len + 1).
+ proof. move => h k k0 klen k_in_bounds; rewrite get_set_if /#. qed.
+
+  abstract theory WSB.
+    type B.
+    op r : int.
+    op _zero : B.
+    op _m_one : B.
+    op _of_list : W8.t list -> B.
+    op (\bits8) : B -> int -> W8.t.
+
+    axiom _gt0_r : 0 < r.
+    axiom _nth_of_list (l: W8.t list) k :
+      size l = r =>
+      _of_list l \bits8 k = nth W8.zero l k.
+    axiom _wordP:
+      forall (w1 w2 : B),
+        (forall (i : int), 0 <= i && i < r => (w1 \bits8 i) = (w2 \bits8 i)) =>
+      w1 = w2.
+    axiom _zero_bits8 i : _zero \bits8 i = W8.zero.
+
+    axiom _m_one_bits8 i :  0<=i < r =>  _m_one \bits8 i = W8.onew.
+
+    op get'Sd (t:t) (i:int) : B =
+      _of_list (sub t i r)
+    axiomatized by get'SdE.
+
+    op set'Sd (t:t) (i:int) (w:B) =
+      fill (fun k => w \bits8 k - i) i r t
+    axiomatized by set'SdE.
+
+
+    abbrev [-printing] get'S (t:t) (i:int) : B = get'Sd t (r * i).
+    abbrev [-printing] set'S (t:t) (i:int) (w:B) = set'Sd t (r * i) w.
+    theory Notation'S.
+      abbrev "_.[_<-_]" = set'S.
+    end Notation'S.
+    export Notation'S.
+
+    lemma get8_set'SdE (t:t) (i:int) (w:B) j :
+      (set'Sd t i w).[j] =
+      if i <= j < i + r /\ 0 <= j && j < ByteArray.size then  w \bits8 (j - i) else t.[j].
+    proof. by rewrite /set'Sd filliEs. qed.
+
+    lemma is_init_cell_set'Sd (t:t) (i j: int):
+        is_init_cell (set'Sd t i _m_one) j = (i <= j < i + r \/ is_init_cell t j).
+    proof.
+      rewrite /is_init_cell get8_set'SdE -oneE /=.
+      smt(_m_one_bits8).
+    qed.
+
+    hint simplify is_init_cell_set'Sd.
+
+    lemma get'Sd_byte (t:t) (i k:int) :
+      0 <= k < r =>
+      get'Sd t i \bits8 k = t.[i+k].
+    proof.
+      case=> hk hr; rewrite /get'Sd _nth_of_list 1:size_map 1:size_iota 1:lez_maxr 3:nth_sub //.
+      move/ltzW: hr.
+      exact: lez_trans hk.
+    qed.
+
+    lemma get_set'SdE (t:t) (i:int) (w:B) j :
+      get'Sd (set'Sd t i w) j =
+      if j + r <= i \/ i + r <= j then get'Sd t j
+      else
+        _of_list
+          (map (fun k => if i <= j + k < i + r /\ 0 <= j + k && j + k < ByteArray.size then
+                            w \bits8 (j + k - i)
+                         else t.[j + k])
+             (iota_ 0 r)).
+    proof.
+      apply _wordP => k hk.
+      rewrite get'Sd_byte 1:// get8_set'SdE.
+      case: (j + r <= i \/ i + r <= j) => hj.
+      + rewrite get'Sd_byte 1://.
+        suff -> : !(i <= j + k < i + r) by done.
+        by case: hj => /#.
+      by rewrite _nth_of_list 1:size_map 1:size_iota 1:/# (nth_map 0) 1:size_iota 1:/# nth_iota.
+    qed.
+
+    lemma get_set'SE_eq t i j w:
+      0 <= i => r*(i + 1) <= ByteArray.size =>
+      i = j =>
+      get'S (set'S t i w) j = w.
+    proof.
+      move=> hx hs <<-; rewrite get_set'SdE.
+      have -> /= : !(r * i + r <= r * i \/ r * i + r <= r * i) by smt(_gt0_r).
+      apply _wordP => k hk.
+      by rewrite _nth_of_list 1:size_map 1:size_iota 1:/# (nth_map 0) 1:size_iota 1:/# /= nth_iota // /#.
+    qed.
+
+    lemma get_set'SE_neq t i j w:
+      i <> j =>
+      get'S (set'S t i w) j = get'S t j.
+    proof.
+      move=> hne; rewrite get_set'SdE.
+      case: (r * j + r <= r * i \/ r * i + r <= r * j) => //.
+      move=> /negb_or [] /ltrNge + /ltrNge.
+      have [-> ->] : r * j + r = r * (j + 1) /\ r * i + r = r * (i + 1) by smt().
+      move=> /(ltr_pmul2l _ _gt0_r) ? /(ltr_pmul2l _ _gt0_r) ? /#.
+    qed.
+
+    lemma get_set'SE t i j w:
+      0 <= i => r*(i + 1) <= ByteArray.size =>
+      get'S (set'S t i w) j = if i = j then w else get'S t j.
+    proof.
+      move=> hx hs.
+      by case (i=j) => heq; [apply get_set'SE_eq | apply get_set'SE_neq].
+    qed.
+
+    lemma get_set'SdE_eq t i j w:
+      0 <= i => i + r <= ByteArray.size =>
+      i = j =>
+      get'Sd (set'Sd t i w) j = w.
+    proof.
+      move=> h1 h2 <<-; rewrite get_set'SdE //.
+      have -> /= : !(i + r <= i) by smt(_gt0_r).
+      apply _wordP => k hk; rewrite _nth_of_list 1:size_map 1:size_iota 1:/# /=.
+      rewrite (nth_map 0) 1:size_iota 1:/# /= nth_iota // /#.
+    qed.
+
+    lemma get_set'SdE_neq t i j w:
+      (j + r <= i \/ i + r <= j) =>
+      get'Sd (set'Sd t i w) j = get'Sd t j.
+    proof. by move => h; rewrite get_set'SdE h. qed.
+
+    hint simplify get_set'SdE_eq, get_set'SdE_neq.
+
+    lemma ext_eq'S t1 t2:
+        (forall x, 0 <= r*x < ByteArray.size => get'S t1 x = get'S t2 x) =>
+        t1 = t2.
+    proof.
+    have ? := _gt0_r.
+    move => E.
+    apply ByteArray.ext_eq => x h.
+    rewrite (divz_eq x r).
+    rewrite !(-get'Sd_byte, modz_cmp, _gt0_r).
+    rewrite mulzC E 2://.
+    smt().
+    qed.
+
+    op of_list'S (l:B list) =
+      init (fun i => if i < List.size l * r then nth _zero l (i%/r) \bits8 (i%%r) else W8.zero).
+
+    lemma get8_of_list'S l i :
+      (of_list'S l).[i] =
+         if (0 <= i < ByteArray.size) /\ i < List.size l * r then nth _zero l (i%/r) \bits8 (i%%r) else W8.zero.
+    proof.
+      rewrite /of_list'S.
+      case: (0 <= i && i < ByteArray.size) => hi; last by rewrite get_out.
+      by rewrite initiE.
+    qed.
+
+    lemma get'S_of_list'S l i :
+      List.size l * r = ByteArray.size =>
+      get'S (of_list'S l) i = nth _zero l i.
+    proof.
+      move=> h; apply _wordP => k hk.
+      rewrite get'Sd_byte // get8_of_list'S.
+      rewrite (mulzC r i) edivz_eq 1:/# emodz_eq 1:/#.
+      case: (0 <= i < List.size l) => hi.
+      + rewrite -h.
+        have -> /= : 0 <= i * r + k by smt().
+        suff -> // : i * r + k < size l * r.
+        suff /# : i * r + (k + 1) <= size l * r.
+        have : (i + 1) * r <= size l * r by apply ler_wpmul2r => /#.
+        apply: ler_trans; smt().
+      rewrite nth_out 1:// _zero_bits8 /#.
+    qed.
+
+  end WSB.
+
+  clone include WSB with
+    type B <- W16.t,
+    op r <- 2,
+    op _zero <- W16.zero,
+    op _m_one <- W16.of_int 65535,
+    op _of_list <- W2u8.pack2,
+    op (\bits8) <- W2u8.(\bits8),
+    axiom _gt0_r <- W2u8.gt0_r,
+    axiom _nth_of_list <- W2u8.get_pack2,
+    axiom _wordP <- W2u8.wordP,
+    axiom _zero_bits8 <- W2u8.get_zero,
+    axiom _m_one_bits8 <- W2u8._m_one_bits8
+  rename [op, lemma, theory] "'S" as "16".
+
+  clone include WSB with
+    type B <- W32.t,
+    op r <- 4,
+    op _zero <- W32.zero,
+    op _m_one <- W32.of_int 4294967295,
+    op _of_list <- W4u8.pack4,
+    op (\bits8) <- W4u8.(\bits8),
+    axiom _gt0_r <- W4u8.gt0_r,
+    axiom _nth_of_list <- W4u8.get_pack4,
+    axiom _wordP <- W4u8.wordP,
+    axiom _zero_bits8 <- W4u8.get_zero,
+    axiom _m_one_bits8 <- W4u8._m_one_bits8
+  rename [op, lemma, theory] "'S" as "32".
+
+  clone include WSB with
+    type B <- W64.t,
+    op r <- 8,
+    op _zero <- W64.zero,
+    op _m_one <- W64.of_int 18446744073709551615,
+    op _of_list <- W8u8.pack8,
+    op (\bits8) <- W8u8.(\bits8),
+    axiom _gt0_r <- W8u8.gt0_r,
+    axiom _nth_of_list <- W8u8.get_pack8,
+    axiom _wordP <- W8u8.wordP,
+    axiom _zero_bits8 <- W8u8.get_zero,
+    axiom _m_one_bits8 <- W8u8._m_one_bits8
+  rename [op, lemma, theory] "'S" as "64".
+
+  clone include WSB with
+    type B <- W128.t,
+    op r <- 16,
+    op _zero <- W128.zero,
+    op _m_one <- W128.of_int 340282366920938463463374607431768211455,
+    op _of_list <- W16u8.pack16,
+    op (\bits8) <- W16u8.(\bits8),
+    axiom _gt0_r <- W16u8.gt0_r,
+    axiom _nth_of_list <- W16u8.get_pack16,
+    axiom _wordP <- W16u8.wordP,
+    axiom _zero_bits8 <- W16u8.get_zero,
+    axiom _m_one_bits8 <- W16u8._m_one_bits8
+  rename [op, lemma, theory] "'S" as "128".
+
+  clone include WSB with
+    type B <- W256.t,
+    op r <- 32,
+    op _zero <- W256.zero,
+    op _m_one <-  W256.of_int 115792089237316195423570985008687907853269984665640564039457584007913129639935,
+    op _of_list <- W32u8.pack32,
+    op (\bits8) <- W32u8.(\bits8),
+    axiom _gt0_r <- W32u8.gt0_r,
+    axiom _nth_of_list <- W32u8.get_pack32,
+    axiom _wordP <- W32u8.wordP,
+    axiom _zero_bits8 <- W32u8.get_zero,
+    axiom _m_one_bits8 <- W32u8._m_one_bits8
+  rename [op, lemma, theory] "'S" as "256".
+
+end ByteArray.
+
+abstract theory SubByteArray.
+
+  clone ByteArray as Asmall.
+  clone ByteArray as Abig.
+
+  op get_sub (a: Abig.t) i : Asmall.t =
+    Asmall.of_list (Abig.sub a i Asmall.size).
+
+  op set_sub (a:Abig.t) (i:int) (s:Asmall.t) =
+    Abig.fill (fun k => Asmall.get8 s (k - i)) i Asmall.size a.
+
+  abbrev [-printing] get_sub8   a i = get_sub a       i.
+  abbrev [-printing] get_sub16  a i = get_sub a ( 2 * i).
+  abbrev [-printing] get_sub32  a i = get_sub a ( 4 * i).
+  abbrev [-printing] get_sub64  a i = get_sub a ( 8 * i).
+  abbrev [-printing] get_sub128 a i = get_sub a (16 * i).
+  abbrev [-printing] get_sub256 a i = get_sub a (32 * i).
+
+  abbrev [-printing] set_sub8   a i s = set_sub a       i  s.
+  abbrev [-printing] set_sub16  a i s = set_sub a ( 2 * i) s.
+  abbrev [-printing] set_sub32  a i s = set_sub a ( 4 * i) s.
+  abbrev [-printing] set_sub64  a i s = set_sub a ( 8 * i) s.
+  abbrev [-printing] set_sub128 a i s = set_sub a (16 * i) s.
+  abbrev [-printing] set_sub256 a i s = set_sub a (32 * i) s.
+
+  lemma get8_get_sub (a:Abig.t) i k :
+    Asmall.get8 (get_sub a i) k =
+     if (0 <= k < Asmall.size) then Abig.get8 a (i+k)
+     else W8.zero.
+  proof.
+    rewrite /get_sub.
+    case : (0 <= k && k < Asmall.size) => [hk | ?]; last by rewrite Asmall.get_out.
+    by rewrite Asmall.get_of_list // Abig.nth_sub.
+  qed.
+
+  lemma get8_set_sub a i s k :
+    Abig.get8 (set_sub a i s) k =
+     if (i <= k < i + Asmall.size) /\ (0 <= k < Abig.size) then Asmall.get8 s (k - i)
+     else Abig.get8 a k.
+  proof. by rewrite Abig.filliEs. qed.
+
+  lemma is_init_cell_get (t: Abig.t) (i j: int):
+      (0 <= i < Asmall.size) => (0 <= j + i < Abig.size) => (Asmall.is_init_cell (get_sub t j) i)  =  Abig.is_init_cell t (j+i).
+  proof. by move => hi hij; rewrite /is_init_cell get8_get_sub hi hij. qed.
+
+  lemma is_init_cell_set  (t1: Abig.t) (t2: Asmall.t) (i j:int):
+    Abig.is_init_cell(set_sub t1 i t2) j =
+      if i <= j < Asmall.size + i /\ 0 <= j < Abig.size then Asmall.is_init_cell t2 (j - i) else  Abig.is_init_cell t1 j.
+  proof. rewrite /is_init_cell get8_set_sub /#. qed.
+
+  abstract theory GETSUB.
+    type B.
+    op r : int.
+    axiom gt0_r : 0 < r.
+    op (\bits8) : B -> int -> W8.t.
+    op small_get : Asmall.t -> int -> B.
+    op big_get : Abig.t -> int -> B.
+    axiom small_get_byte (t : Asmall.t) (i k : int) :
+      0 <= k && k < r => small_get t i \bits8 k = Asmall.get8 t (i + k).
+    axiom big_get_byte (t : Abig.t) (i k : int) :
+      0 <= k && k < r => big_get t i \bits8 k = Abig.get8 t (i + k).
+    axiom _wordP:
+      forall (w1 w2 : B),
+        (forall (i : int), 0 <= i && i < r => (w1 \bits8 i) = (w2 \bits8 i)) =>
+      w1 = w2.
+
+    lemma get'Sd_get_sub_byte (a:Abig.t) i k j :
+      0 <= j < r =>
+      (small_get (get_sub a i) k) \bits8 j =
+      if 0 <= k + j && k + j < Asmall.size then Abig.get8 a (i + k + j)
+      else W8.zero.
+    proof. move=> hj; rewrite small_get_byte 1:// get8_get_sub /#. qed.
+
+    lemma get'Sd_get_sub (a:Abig.t) i k :
+      (0 <= k /\ k + r <= Asmall.size) =>
+      small_get (get_sub a i) k = big_get a (i+k).
+    proof.
+      move=> hk; apply _wordP => j jh.
+      rewrite get'Sd_get_sub_byte 1:// big_get_byte 1:// /#.
+    qed.
+
+    lemma get'Sd_set_sub_byte (a:Abig.t) (i k:int) s j :
+      0 <= j < r =>
+      big_get (set_sub a i s) k \bits8 j =
+       if (i <= k + j < i + Asmall.size) /\ (0 <= k + j < Abig.size) then Asmall.get8 s (k + j - i)
+       else Abig.get8 a (k + j).
+    proof. by move=> hj; rewrite big_get_byte 1:// get8_set_sub. qed.
+
+    lemma get'Sd_set_sub_in (a:Abig.t) (i k:int) s :
+      (0 <= i /\ i + Asmall.size <= Abig.size) /\
+      (0 <= k - i /\ k - i + r <= Asmall.size) =>
+      big_get (set_sub a i s) k = small_get s (k - i).
+    proof.
+      move=> h; apply _wordP => j hj.
+      rewrite get'Sd_set_sub_byte 1:// small_get_byte 1:// /#.
+    qed.
+
+    lemma get'Sd_set_sub_out (a:Abig.t) (i k:int) s :
+      (0 <= i /\ i + Asmall.size <= Abig.size) /\
+      (k + r <= i \/ i + Asmall.size <= k) =>
+      big_get (set_sub a i s) k = big_get a k.
+    proof.
+      move=> h; apply _wordP => j hj.
+      rewrite get'Sd_set_sub_byte 1:// big_get_byte 1:// /#.
+    qed.
+
+  end GETSUB.
+
+  clone include GETSUB with
+    type B <- W16.t,
+    op r <- 2,
+    axiom gt0_r <- W2u8.gt0_r,
+    op (\bits8) <- W2u8.(\bits8),
+    op small_get <- Asmall.get16d,
+    op big_get <- Abig.get16d,
+    axiom small_get_byte <- Asmall.get16d_byte,
+    axiom big_get_byte <- Abig.get16d_byte,
+    axiom _wordP <- W2u8.wordP
+  rename [op, lemma] "'S" as "16".
+
+  clone include GETSUB with
+    type B <- W32.t,
+    op r <- 4,
+    axiom gt0_r <- W4u8.gt0_r,
+    op (\bits8) <- W4u8.(\bits8),
+    op small_get <- Asmall.get32d,
+    op big_get <- Abig.get32d,
+    axiom small_get_byte <- Asmall.get32d_byte,
+    axiom big_get_byte <- Abig.get32d_byte,
+    axiom _wordP <- W4u8.wordP
+  rename [op, lemma] "'S" as "32".
+
+  clone include GETSUB with
+    type B <- W64.t,
+    op r <- 8,
+    axiom gt0_r <- W8u8.gt0_r,
+    op (\bits8) <- W8u8.(\bits8),
+    op small_get <- Asmall.get64d,
+    op big_get <- Abig.get64d,
+    axiom small_get_byte <- Asmall.get64d_byte,
+    axiom big_get_byte <- Abig.get64d_byte,
+    axiom _wordP <- W8u8.wordP
+  rename [op, lemma] "'S" as "64".
+
+  clone include GETSUB with
+    type B <- W128.t,
+    op r <- 16,
+    axiom gt0_r <- W16u8.gt0_r,
+    op (\bits8) <- W16u8.(\bits8),
+    op small_get <- Asmall.get128d,
+    op big_get <- Abig.get128d,
+    axiom small_get_byte <- Asmall.get128d_byte,
+    axiom big_get_byte <- Abig.get128d_byte,
+    axiom _wordP <- W16u8.wordP
+  rename [op, lemma] "'S" as "128".
+
+  clone include GETSUB with
+    type B <- W256.t,
+    op r <- 32,
+    axiom gt0_r <- W32u8.gt0_r,
+    op (\bits8) <- W32u8.(\bits8),
+    op small_get <- Asmall.get256d,
+    op big_get <- Abig.get256d,
+    axiom small_get_byte <- Asmall.get256d_byte,
+    axiom big_get_byte <- Abig.get256d_byte,
+    axiom _wordP <- W32u8.wordP
+  rename [op, lemma] "'S" as "256".
+
+end SubByteArray.
+
+
+
+
+
